ulib/LowStar.Modifies.fsti
@@ -442,20 +442,9 @@ val modifies_mreference_elim
     [ SMTPat (modifies p h h'); SMTPat (HS.contains h' b) ]
   ] ]
 
-/// If a buffer ``b`` *of positive length* is disjoint from a set ``p`` of
+/// If a buffer ``b`` is disjoint from a set ``p`` of
 /// memory locations which is modified, then its liveness and contents
 /// are preserved.
-///
-/// Here it is important to require that the length of ``b`` must not be
-/// zero. Indeed, let ``x`` be a buffer of size 2, and pose ``y = B.gsub
-/// x 2ul 0ul``. Then, ``y`` is disjoint from ``x``, because it is a
-/// sub-buffer of ``x`` covering a range disjoint from that of ``x``
-/// (since ``x == B.gsub x 0ul 2ul``.) However, if ``x`` is deallocated,
-/// then ``x`` is no longer live, and so neither is ``y``, as a sub-buffer
-/// of ``x``. This means that the liveness of buffers of length 0 cannot
-/// be preserved by modifies clauses. Fortunately, in most cases, to
-/// talk about the liveness of ``y``, it is always possible to reason
-/// about the liveness of a buffer which encloses ``y``, such as ``x``.
 
 val modifies_buffer_elim
   (#t1: Type)
@@ -466,7 +455,6 @@ val modifies_buffer_elim
   (requires (
     loc_disjoint (loc_buffer b) p /\
     B.live h b /\
-    ((B.length b) == 0 ==> B.live h' b) /\ // necessary for liveness, because all buffers of size 0 are disjoint for any memory location, so we cannot talk about their liveness individually without referring to a larger nonempty buffer
     modifies p h h'
   ))
   (ensures (
@@ -646,7 +634,7 @@ val modifies_0_modifies
     [SMTPat (modifies loc_none h1 h2)];
   ]]
 
-/// Case ``modifies_1``: update, free.
+/// Case ``modifies_1``: update.
 
 val modifies_1_modifies
   (#a: Type)
@@ -659,6 +647,18 @@ val modifies_1_modifies
     [SMTPat (B.modifies_1 b h1 h2)];
     [SMTPat (modifies (loc_buffer b) h1 h2)];
   ]]
+
+/// Case ``modifies_addr_of``: free. 
+
+val modifies_addr_of_modifies
+  (#a: Type)
+  (b: B.buffer a)
+  (h1 h2: HS.mem)
+: Lemma
+  (requires (B.modifies_addr_of b h1 h2))
+  (ensures (modifies (loc_addresses (B.frameOf b) (Set.singleton (B.as_addr b))) h1 h2))
+  [SMTPat (B.modifies_addr_of b h1 h2)]
+
 
 /// Any live reference is disjoint from a buffer which has not been allocated yet.
 
